\begin{mathexam}{\(\scalerel{\int}{\dfrac{6^{x-1} + 4^{x+1}}{2^x}}\dd{x}\)}{exam147} 
  Integrand postupně převedeme na součet dvou funkcí:
  \begin{multline*}
    \dfrac{6^{x-1} + 4^{x+1}}{2^x} = \dfrac{6^{-1}\cdot6^x + 4\cdot4^x}{2^x} =   \\
      = \dfrac{6^{-1}\cdot\cancel{2^x}\cdot3^x + 4\cdot\cancel{2^x}\cdot2^x}{\cancel{2^x}} 
      = 6^{-1}\cdot3^x + 4\cdot2^x. 
  \end{multline*}
  Použitím věty \ref{mai:lemma013} dostaneme
  \begin{multline*}
    \int\left(\dfrac{6^{x-1}+4^{x+1}}{2^x}\right)\dd{x} = \int(6^{-1}\cdot3^x + 4\cdot2^x)\dd{x} \\
      = \dfrac{1}{6\ln3}3^x + \dfrac{4}{\ln2}2^x + c
  \end{multline*}
\end{mathexam}